PropositionalLogic/TrivialSemantics.v
@@ -1,6 +1,5 @@
 Require Import Coq.Logic.Classical_Prop.
 Require Import Logic.MinimunLogic.LogicBase.
-Require Import Logic.MinimunLogic.MinimunLogic.
 Require Import Logic.PropositionalLogic.Syntax.
 
 Local Open Scope logic_base.
